theories/iris/examples/effects/generator_module.v
@@ -44,7 +44,10 @@ Section GeneratorModule.
       mod_start := None;
       mod_imports := [];
       mod_exports := [
-        {| modexp_name := String.list_byte_of_string "generator function" ;
+        {| modexp_name := String.list_byte_of_string "generator tag";
+          modexp_desc :=
+            MED_tag (Mk_tagidx 0) |} ;
+        {| modexp_name := String.list_byte_of_string "naturals function" ;
           modexp_desc :=
             MED_func (Mk_funcidx 0) |} ;
         {| modexp_name := String.list_byte_of_string "sum_until function" ;
@@ -54,7 +57,7 @@ Section GeneratorModule.
       mod_tags := [tag_type]
     |}.
 
-  Definition expts := [ET_func naturals_type ; ET_func sum_until_type].
+  Definition expts := [ET_tag tag_type; ET_func naturals_type ; ET_func sum_until_type].
 
   Lemma coroutines_module_typing :
     module_typing generator_module [] expts.
@@ -65,26 +68,29 @@ Section GeneratorModule.
     - rewrite ! Forall2_cons. repeat split;auto; cbn;auto.
         apply naturals_typing.
         apply sum_until_typing.
-    - constructor => //. constructor => //.
+    - constructor => //. constructor => //. constructor => //.
   Qed.
 
-  Definition generator_module_instantiate naturals_exp_addr sum_until_exp_addr mod_addr:=
-    [ ID_instantiate [ naturals_exp_addr ; sum_until_exp_addr ] mod_addr [] ].
+  Definition generator_module_instantiate tag_exp_addr naturals_exp_addr sum_until_exp_addr mod_addr:=
+    [ ID_instantiate [ tag_exp_addr ; naturals_exp_addr ; sum_until_exp_addr ] mod_addr [] ].
 
   Notation "{{{{ P }}}} es {{{{ v , Q }}}}" :=
     (□ ∀ Φ, P -∗ (∀ v, Q -∗ Φ v) -∗ WP (es : host_expr) @ NotStuck ; ⊤ {{ v, Φ v }})%I (at level 50).
 
-  Lemma instantiate_generator naturals_exp_addr sum_until_exp_addr mod_addr:
+  Lemma instantiate_generator tag_exp_addr naturals_exp_addr sum_until_exp_addr mod_addr:
     ⊢ {{{{
               mod_addr ↪[mods] generator_module ∗
+                (∃ exp0, tag_exp_addr ↪[vis] exp0) ∗
                 (∃ exp1, naturals_exp_addr ↪[vis] exp1) ∗
                 (∃ exp2, sum_until_exp_addr ↪[vis] exp2)
       }}}}
-      ((generator_module_instantiate naturals_exp_addr sum_until_exp_addr mod_addr,
-         [], empty_frame) : host_expr) 
+      ((generator_module_instantiate tag_exp_addr naturals_exp_addr sum_until_exp_addr mod_addr,
+         [], empty_frame) : host_expr)
         {{{{  x,  ⌜x = (immHV [], empty_frame)⌝ ∗
                           mod_addr ↪[mods] generator_module ∗
-                          ∃ addr_naturals addr_sum_until addr_tag name_naturals name_sum_until cl_naturals cl_sum_until,
+                          ∃ addr_naturals addr_sum_until addr_tag name_tag name_naturals name_sum_until cl_naturals cl_sum_until,
+                            tag_exp_addr ↪[vis] {| modexp_name := name_tag;
+                                                    modexp_desc := MED_tag (Mk_tagidx addr_tag) |} ∗
                             naturals_exp_addr ↪[vis] {| modexp_name := name_naturals;
                                                     modexp_desc := MED_func (Mk_funcidx addr_naturals) |} ∗
                             sum_until_exp_addr ↪[vis] {| modexp_name := name_sum_until;
@@ -97,11 +103,11 @@ Section GeneratorModule.
 
                             (∀ I, ∃ Ψ, naturals_spec addr_tag addr_naturals cl_naturals Ψ I) ∗
                             sum_until_spec addr_tag addr_naturals addr_sum_until cl_naturals cl_sum_until
-        }}}} .
+        }}}}.
   Proof.
-    iIntros "!>" (Φ) "(Hmod & Hvis1 & Hvis2) HΦ".
+    iIntros "!>" (Φ) "(Hmod & Hvis0 & Hvis1 & Hvis2) HΦ".
     iApply (weakestpre.wp_wand _ _ (_ : host_expr) with "[- HΦ]").
-    iApply (instantiation_spec_operational_no_start with "[$Hmod Hvis1 Hvis2]") => //.
+    iApply (instantiation_spec_operational_no_start with "[$Hmod Hvis0 Hvis1 Hvis2]") => //.
     - apply coroutines_module_typing.
     - unfold module_restrictions. cbn. repeat split;exists [];auto.
     - iFrame.
@@ -124,7 +130,7 @@ Section GeneratorModule.
       iSplit; first done.
       unfold instantiation_resources_post.
       iDestruct "H" as "(Hmod & Himports & %inst & Hresources & Hexports)".
-      iDestruct "Hexports" as "([%name1 Hexp1] & [%name2 Hexp2] & _)".
+      iDestruct "Hexports" as "([%name0 Hexp0] & [%name1 Hexp1] & [%name2 Hexp2] & _)".
       simpl.
       iFrame.
       unfold instantiation_resources_post_wasm.
@@ -166,6 +172,6 @@ Section GeneratorModule.
       iApply naturals_spec_proof.
       by unfold closure_naturals, generator_inst.
   Qed.
-    
-    
+
+
 End GeneratorModule.
